# Aufgabe 89
## Angabe

Es sei $\displaystyle \lim_{n \to \infin} a_n = a$. Man bestimme den Grenzwert der Reihe $\displaystyle \sum_{n \ge  0}(a_{n+1} - a_n)$.

## Lösungsweg

### Partialsumme

$\displaystyle s_n = (a_1 - a_0) + (a_2 - a_1) + (a_3 - a_2) + ... + (a_{n+1} - a_{n})$

Das ist eine Teleskopsumme, bei der sich benachbarte Terme gegenseitig aufheben

$s_n = a_{n+1} - a_0$

### Konvergenz

$\displaystyle \lim_{n \to \infin} s_n = \lim_{n \to \infin}(a_{n+1} - a_0) = a - a_0$

$\displaystyle \sum_{n \ge  0}(a_{n+1} − a_n) = a - a_0$