# Aufgabe 325
## Angabe

Es sei $\color{orange}g_u(u,v)=\frac{\partial}{\partial_u}g(u,v)=(1-2u^2)e^{-u^2+v^3}$ und $\color{magenta}g_v(u,v)=\frac{\partial}{\partial_v}g(u,v)=3uv^2e^{-u^2+v^3}$. 

Man bestimme mit Hilfe der Kettenregel $h(t)=\frac{d}{dt}g(\textcolor{green}{t^2-1},\textcolor{teal}{3t})$. 

## Hilfreiches

**Satz 6.20 (Kettenregel)**

Sei $D \subseteq \R^n$ eine offene Menge, $f: D \to \R$ und $g: \R \to \R^n$ mit $g(x)=(g_1(x), \dots, g_n(x))$ und $g(\R) \subseteq D$. Weiters sei $F(x)=f(g(x))$. Dann gilt

$\displaystyle F'(x)=\sum_{i=1}^n f_{x_i}(g_1(x), …, g_n(x)) g_i'(x)$

In Leibniz'scher Notation:

$\displaystyle \frac{dF}{dx}=\sum_{i=1}^n \frac{\partial f}{\partial g_i}\cdot \frac{d g_i}{dx}$

## Lösungsvorschlag

$\displaystyle \frac{dg}{dt}=\sum_{i=1}^2 \frac{\partial g}{\partial g_i}\cdot \frac{d g_i}{dt}=\quad\textcolor{orange}{\frac{\partial g}{\partial u}}\cdot \textcolor{springgreen}{\frac{d u}{dt}}+\textcolor{magenta}{\frac{\partial g}{\partial v}}\cdot \textcolor{cyan}{\frac{d v}{dt}}$

$\color{orange} g_u(u,v)=\frac{\partial}{\partial_u}g(u,v)=(1-2u^2)e^{-u^2+v^3}$ \
$\color{magenta}g_v(u,v)=\frac{\partial}{\partial_v}g(u,v)=3uv^2e^{-u^2+v^3}$

$\color{green}u=t^2-1$ \
$\color{teal}v=3t$

$\color{springgreen}\frac{du}{dt}=u'=2t$ \
$\color{cyan}\frac{dv}{dt}=v'=3$

$h(t)=\textcolor{orange}{(1-2u^2)e^{-u^2+v^3}}\cdot \textcolor{springgreen}{2t}+\textcolor{magenta}{3uv^2e^{-u^2+v^3}}\cdot \textcolor{cyan}{3}$

$=\textcolor{orange}{(1-2\textcolor{green}{(t^2-1)}^2)e^{-\textcolor{green}{(t^2-1)}^2+\textcolor{teal}{(3t)}^3}}\cdot \textcolor{springgreen}{2t}+\textcolor{magenta}{3\textcolor{green}{(t^2-1)}\textcolor{teal}{(3t)}^2e^{-\textcolor{green}{(t^2-1)}^2+\textcolor{teal}{(3t)}^3}}\cdot \textcolor{cyan}{3}$

$=\textcolor{orange}{(1-2(t^4-2t^2+1))e^{-(t^4-2t^2+1)+(27t^3)}}\cdot \textcolor{springgreen}{2t}+\textcolor{magenta}{3\textcolor{green}{(t^2-1)}(9t^2)e^{-(t^4-2t^2+1)+(27t^3)}}\cdot \textcolor{cyan}{3}$

$=\textcolor{orange}{(-2t^4+4t^2-1)e^{-t^4+27t^3+2t^2-1}}\cdot \textcolor{springgreen}{2t}+\textcolor{magenta}{(27t^4-27t^2)e^{-t^4+27t^3+2t^2-1}}\cdot \textcolor{cyan}{3}$

$h(t)=e^{-t^4+27t^3+2t^2-1}((-2t^4+4t^2-1)\cdot 2t+(27t^4-27t^2)\cdot 3)$